@prefix : <https://w3id.org/aidoc-ap#> .
@base <https://w3id.org/aidoc-ap#> .

@prefix owl: <http://www.w3.org/2002/07/owl#> .
@prefix rdf: <http://www.w3.org/1999/02/22-rdf-syntax-ns#> .
@prefix xml: <http://www.w3.org/XML/1998/namespace> .
@prefix xsd: <http://www.w3.org/2001/XMLSchema#> .
@prefix rdfs: <http://www.w3.org/2000/01/rdf-schema#> .
@prefix dcterms: <http://purl.org/dc/terms/> .
@prefix foaf: <http://xmlns.com/foaf/0.1/> .
@prefix skos: <http://www.w3.org/2004/02/skos/core#> .
@prefix vann: <http://purl.org/vocab/vann/> .
@prefix schema: <https://schema.org/> .
@prefix widoco: <https://w3id.org/widoco/vocab#> .
@prefix bibo: <http://purl.org/ontology/bibo/> .


#################################################################
#    Ontology Metadata 
#################################################################

<https://w3id.org/aidoc-ap#>
    rdf:type owl:Ontology ;
    dcterms:title "AIDOC-AP - AI Documentation Application Profile"@en ;
    dcterms:description "The AI Documentation Application Profile (AIDOC-AP) is designed to provide a structured, machine-readable model of an AI system and its entire lifecycle. It is built as a modular framework, rooted in established semantic web standards and enhanced with domain-specific concepts from the research material provided. The core of AIDOC-AP is a graph-based representation that captures the provenance of all AI artifacts, the activities that create and modify them, and the agents responsible for those activities."@en ;
    dcterms:creator [
        rdf:type foaf:Person ;
        foaf:name "Sebastian Neumaier" ;
        foaf:mbox <mailto:sebastian.neumaier@ustp.at> ;
        foaf:organization "University of Applied Sciences St. Pölten"
    ], [
        rdf:type foaf:Person ;
        foaf:name "Fabian Kovac" ;
        foaf:mbox <mailto:fabian.kovac@ustp.at> ;
        foaf:organization "University of Applied Sciences St. Pölten"
    ], [
        rdf:type foaf:Person ;
        foaf:name "Timea Pahi" ;
        foaf:mbox <mailto:timea.pahi@ustp.at> ;
        foaf:organization "University of Applied Sciences St. Pölten"
    ] ;
    dcterms:publisher [
        foaf:name "CERTAIN Project" ;
        foaf:homepage <https://certain-project.eu> 
    ] ;
    dcterms:issued "2025-11-11"^^xsd:date ;
    owl:versionInfo "1.0" ;
    dcterms:license <https://creativecommons.org/licenses/by/4.0/> ;
    vann:preferredNamespacePrefix "aidoc" ;
    vann:preferredNamespaceUri "https://w3id.org/aidoc-ap#" ;
    schema:keywords "AI systems, ontology, AIDOC-AP, AI lifecycle, AI Act"@en ;
    schema:funding <https://cordis.europa.eu/project/id/101189650> ;
    dcterms:language "en" ;
    rdfs:label "AIDOC-AP"@en ;
    owl:versionIRI <https://w3id.org/aidoc-ap/1.0> .
 

#################################################################
#    Annotation properties
#################################################################

###  http://www.w3.org/2004/02/skos/core#closeMatch
<http://www.w3.org/2004/02/skos/core#closeMatch> rdf:type owl:AnnotationProperty .


#################################################################
#    Object Properties
#################################################################

###  http://purl.org/dc/terms/hasPart
<http://purl.org/dc/terms/hasPart> rdf:type owl:ObjectProperty .


###  https://w3id.org/aidoc-ap#hasCapability
<https://w3id.org/aidoc-ap#hasCapability> rdf:type owl:ObjectProperty ;
                                                          rdfs:domain <https://w3id.org/aidoc-ap#AISystem> ;
                                                          rdfs:range <https://w3id.org/aidoc-ap#AISystemCapability> ;
                                                          rdfs:comment "Relates an AISystem to an AISystemCapability it is designed to exhibit or support" ;
                                                          rdfs:label "has capability"@en .


###  https://w3id.org/aidoc-ap#implementsTask
<https://w3id.org/aidoc-ap#implementsTask> rdf:type owl:ObjectProperty ;
                                            rdfs:domain <https://w3id.org/aidoc-ap#AIMethod> ;
                                            rdfs:range <https://w3id.org/aidoc-ap#AITask> ;
                                            rdfs:comment "Links an AIMethod to the AITask it is designed to perform."@en ;
                                            rdfs:label "implements task"@en .


###  https://w3id.org/aidoc-ap#supportsCapability
<https://w3id.org/aidoc-ap#supportsCapability> rdf:type owl:ObjectProperty ;
                                               rdfs:domain <https://w3id.org/aidoc-ap#AITask> ;
                                               rdfs:range <https://w3id.org/aidoc-ap#AISystemCapability> ;
                                               rdfs:comment "Indicates that an AITask contributes to achieving a broader AISystemCapability."@en ;
                                               rdfs:label "supports capability"@en .


###  https://w3id.org/aidoc-ap#appliesStandard
<https://w3id.org/aidoc-ap#appliesStandard> rdf:type owl:ObjectProperty ;
                                            rdfs:domain <https://w3id.org/aidoc-ap#AISystem> ;
                                            rdfs:range <https://w3id.org/aidoc-ap#Standard> ;
                                            rdfs:comment "Links an AI system to a standard it has applied for compliance."@en ;
                                            rdfs:label "applies standard"@en .


###  https://w3id.org/aidoc-ap#dependsOn
<https://w3id.org/aidoc-ap#dependsOn> rdf:type owl:ObjectProperty ;
                                      rdfs:subPropertyOf <http://purl.org/dc/terms/hasPart> ;
                                      rdfs:domain <https://w3id.org/aidoc-ap#AISystem> ;
                                      rdfs:range <https://w3id.org/aidoc-ap#AI_Artifact> ;
                                      rdfs:comment "Links a system or component to its software or hardware dependencies."@en ;
                                      rdfs:label "depends on"@en .


###  https://w3id.org/aidoc-ap#hasComponent
<https://w3id.org/aidoc-ap#hasComponent> rdf:type owl:ObjectProperty ;
                                         rdfs:domain <https://w3id.org/aidoc-ap#AISystem> ;
                                         rdfs:range <https://w3id.org/aidoc-ap#AI_Artifact> ;
                                         rdfs:comment "Links an AISystem to its constituent components like models and datasets."@en ;
                                         rdfs:label "has component"@en .


###  https://w3id.org/aidoc-ap#hasDeclarationOfConformity
<https://w3id.org/aidoc-ap#hasDeclarationOfConformity> rdf:type owl:ObjectProperty ;
                                                       rdfs:domain <https://w3id.org/aidoc-ap#AISystem> ;
                                                       rdfs:range <https://w3id.org/aidoc-ap#DeclarationOfConformity> ;
                                                       rdfs:comment "Links an AI system to its EU Declaration of Conformity document."@en ;
                                                       rdfs:label "has declaration of conformity"@en .


###  https://w3id.org/aidoc-ap#hasHumanOversight
<https://w3id.org/aidoc-ap#hasHumanOversight> rdf:type owl:ObjectProperty ;
                                              rdfs:domain <https://w3id.org/aidoc-ap#AISystem> ;
                                              rdfs:range <https://w3id.org/aidoc-ap#HumanOversightMechanism> ;
                                              rdfs:comment "Links an AI system to a mechanism for human oversight or intervention."@en ;
                                              rdfs:label "has human oversight"@en .


###  https://w3id.org/aidoc-ap#hasInterface
<https://w3id.org/aidoc-ap#hasInterface> rdf:type owl:ObjectProperty ;
                                         rdfs:domain <https://w3id.org/aidoc-ap#AISystem> ;
                                         rdfs:range <https://w3id.org/aidoc-ap#Interface> ;
                                         rdfs:comment "Links an AI system to the interface it provides to users or operators."@en ;
                                         rdfs:label "has interface"@en .


###  https://w3id.org/aidoc-ap#hasLifecycleStage
<https://w3id.org/aidoc-ap#hasLifecycleStage> rdf:type owl:ObjectProperty ;
                                              rdfs:domain <https://w3id.org/aidoc-ap#AISystem> ;
                                              rdfs:range <https://w3id.org/aidoc-ap#AI_Activity> ;
                                              rdfs:comment "Links an AISystem to a specific AI_Activity."@en ;
                                              rdfs:label "has lifecycle stage"@en .


###  https://w3id.org/aidoc-ap#hasPerformanceMetric
<https://w3id.org/aidoc-ap#hasPerformanceMetric> rdf:type owl:ObjectProperty ;
                                                 rdfs:domain <https://w3id.org/aidoc-ap#ModelEvaluation> ;
                                                 rdfs:range <https://w3id.org/aidoc-ap#PerformanceMetric> ;
                                                 rdfs:comment "Links an evaluation activity to the performance metric it uses."@en ;
                                                 rdfs:label "has performance metric"@en .


###  https://w3id.org/aidoc-ap#hasRisk
<https://w3id.org/aidoc-ap#hasRisk> rdf:type owl:ObjectProperty ;
                                    rdfs:domain <https://w3id.org/aidoc-ap#AI_Artifact> ;
                                    rdfs:range <https://w3id.org/airo#AIRisk> ;
                                    rdfs:comment "Links an AI artifact (e.g., model or dataset) or an AI system to an associated risk."@en ;
                                    rdfs:label "has risk"@en .


###  https://w3id.org/aidoc-ap#hasTransparencyMeasure
<https://w3id.org/aidoc-ap#hasTransparencyMeasure> rdf:type owl:ObjectProperty ;
                                                   rdfs:domain <https://w3id.org/aidoc-ap#AISystem> ;
                                                   rdfs:range <https://w3id.org/aidoc-ap#TransparencyMeasure> ;
                                                   rdfs:comment "Links an AI system to measures in place to ensure transparency."@en ;
                                                   rdfs:label "has transparency measure"@en .


###  https://w3id.org/aidoc-ap#isDeployedBy
<https://w3id.org/aidoc-ap#isDeployedBy> rdf:type owl:ObjectProperty ;
                                         rdfs:domain <https://w3id.org/aidoc-ap#AISystem> ;
                                         rdfs:range <https://w3id.org/aidoc-ap#AIDeployer> ;
                                         rdfs:comment "Links an AI system to its deployer."@en ;
                                         rdfs:label "is deployed by"@en .


###  https://w3id.org/aidoc-ap#isProvidedBy
<https://w3id.org/aidoc-ap#isProvidedBy> rdf:type owl:ObjectProperty ;
                                         rdfs:domain <https://w3id.org/aidoc-ap#AISystem> ;
                                         rdfs:range <https://w3id.org/aidoc-ap#AIProvider> ;
                                         rdfs:comment "Links an AI system to its provider."@en ;
                                         rdfs:label "is provided by"@en .


###  https://w3id.org/aidoc-ap#logsActivity
<https://w3id.org/aidoc-ap#logsActivity> rdf:type owl:ObjectProperty ;
                                         rdfs:domain <https://w3id.org/aidoc-ap#DataMonitoringAndLogging> ;
                                         rdfs:range <http://www.w3.org/ns/prov#Activity> ;
                                         rdfs:comment "Links a monitoring activity to the type of activity that is logged."@en ;
                                         rdfs:label "logs activity"@en .


###  https://w3id.org/aidoc-ap#requiresHardware
<https://w3id.org/aidoc-ap#requiresHardware> rdf:type owl:ObjectProperty ;
                                             rdfs:domain <https://w3id.org/aidoc-ap#AISystem> ;
                                             rdfs:range <https://w3id.org/aidoc-ap#HardwareComponent> ;
                                             rdfs:comment "Links a system to the hardware components it needs to run."@en ;
                                             rdfs:label "requires hardware"@en .


###  https://w3id.org/aidoc-ap#storesLogsAt
<https://w3id.org/aidoc-ap#storesLogsAt> rdf:type owl:ObjectProperty ;
                                         rdfs:domain <https://w3id.org/aidoc-ap#DataMonitoringAndLogging> ;
                                         rdfs:range <http://www.w3.org/ns/prov#Entity> ;
                                         rdfs:comment "Links a monitoring activity to where its logs are stored."@en ;
                                         rdfs:label "stores logs at"@en .


###  https://w3id.org/aidoc-ap#usesAIMethod
<https://w3id.org/aidoc-ap#usesAIMethod> rdf:type owl:ObjectProperty ;
                                          rdfs:domain <https://w3id.org/aidoc-ap#AI_Model> ;
                                          rdfs:range <https://w3id.org/aidoc-ap#AIMethod> ;
                                          rdfs:comment "Links an AI model to the specific AI method it is based on."@en ;
                                          rdfs:label "uses AI method"@en .


#################################################################
#    Data properties
#################################################################

###  https://w3id.org/aidoc-ap#evaluationMethod
<https://w3id.org/aidoc-ap#evaluationMethod> rdf:type owl:DatatypeProperty ;
                                             rdfs:domain <https://w3id.org/aidoc-ap#ModelEvaluation> ;
                                             rdfs:range xsd:string ;
                                             rdfs:comment "The methodology used to evaluate a performance metric."@en ;
                                             rdfs:label "evaluation method"@en .


###  https://w3id.org/aidoc-ap#frequency
<https://w3id.org/aidoc-ap#frequency> rdf:type owl:DatatypeProperty ;
                                      rdfs:domain <https://w3id.org/aidoc-ap#AI_Activity> ;
                                      rdfs:range xsd:string ;
                                      rdfs:comment "The frequency with which an activity (e.g., risk re-evaluation) is performed."@en ;
                                      rdfs:label "frequency"@en .


###  https://w3id.org/aidoc-ap#hasArchitecture
<https://w3id.org/aidoc-ap#hasArchitecture> rdf:type owl:DatatypeProperty ;
                                            rdfs:comment "Links a system or model to a description of its architecture."@en ;
                                            rdfs:label "has architecture"@en ;
                                            rdfs:range rdfs:Literal ;
                                            rdfs:domain <https://w3id.org/aidoc-ap#AI_Model> ,
                                                        <https://w3id.org/aidoc-ap#AISystem> .


###  https://w3id.org/aidoc-ap#intendedPurpose
<https://w3id.org/aidoc-ap#intendedPurpose> rdf:type owl:DatatypeProperty ;
                                            rdfs:domain <https://w3id.org/aidoc-ap#AISystem> ;
                                            rdfs:range xsd:string ;
                                            rdfs:comment "The intended purpose of the AI system, as per the AI Act."@en ;
                                            rdfs:label "intended purpose"@en .


###  https://w3id.org/aidoc-ap#modality
<https://w3id.org/aidoc-ap#modality> rdf:type owl:DatatypeProperty ;
                                     rdfs:domain <https://w3id.org/aidoc-ap#AISystem> ;
                                     rdfs:range xsd:string ;
                                     rdfs:comment "The physical form or modality in which the AI system is provided (e.g., standalone software, API)."@en ;
                                     rdfs:label "modality"@en .


###  https://w3id.org/aidoc-ap#version
<https://w3id.org/aidoc-ap#version> rdf:type owl:DatatypeProperty ;
                                    rdfs:domain <http://www.w3.org/ns/prov#Entity> ;
                                    rdfs:range xsd:string ;
                                    rdfs:comment "The version of the AI system or artifact."@en ;
                                    rdfs:label "version"@en .


#################################################################
#    Classes
#################################################################

###  http://mlcommons.org/croissant/1.0#Dataset
<http://mlcommons.org/croissant/1.0#Dataset> rdf:type owl:Class .


###  https://w3id.org/aidoc-ap#AISystemCapability
<https://w3id.org/aidoc-ap#AISystemCapability> rdf:type owl:Class ;
                                               rdfs:comment "Represents a category of tasks or functions that an AI system can perform, such as sensory, knowledge, or control action processing."@en ;
                                               rdfs:label "AI System Capability"@en .


### https://w3id.org/aidoc-ap#AITask
<https://w3id.org/aidoc-ap#AITask> rdf:type owl:Class ;
                                   rdfs:comment "An action to achieve a specific goal using an AI model."@en ;
                                   rdfs:label "AI Task"@en .


###  https://w3id.org/aidoc-ap#AIMethodCategory
<https://w3id.org/aidoc-ap#AIMethodCategory> a rdfs:Class ;
    rdfs:label "AI Method Category" ;
    rdfs:comment "A conceptual grouping of AI methods based on shared characteristics, such as machine learning, search optimization, or knowledge representation."@en .


###  http://www.w3.org/ns/dqv#Metric
<http://www.w3.org/ns/dqv#Metric> rdf:type owl:Class .


###  http://www.w3.org/ns/mls#Dataset
<http://www.w3.org/ns/mls#Dataset> rdf:type owl:Class .


###  http://www.w3.org/ns/mls#Algorithm
<http://www.w3.org/ns/mls#Algorithm> rdf:type owl:Class .


###  http://www.w3.org/ns/mls#Experiment
<http://www.w3.org/ns/mls#Experiment> rdf:type owl:Class .


###  http://www.w3.org/ns/mls#Implementation
<http://www.w3.org/ns/mls#Implementation> rdf:type owl:Class .


###  http://www.w3.org/ns/mls#Model
<http://www.w3.org/ns/mls#Model> rdf:type owl:Class .


###  http://www.w3.org/ns/mls#Software
<http://www.w3.org/ns/mls#Software> rdf:type owl:Class .


###  http://www.w3.org/ns/prov#Activity
<http://www.w3.org/ns/prov#Activity> rdf:type owl:Class .


###  http://www.w3.org/ns/prov#Agent
<http://www.w3.org/ns/prov#Agent> rdf:type owl:Class .


###  http://www.w3.org/ns/prov#Entity
<http://www.w3.org/ns/prov#Entity> rdf:type owl:Class .


###  http://xmlns.com/foaf/0.1/Organization
<http://xmlns.com/foaf/0.1/Organization> rdf:type owl:Class .


###  http://xmlns.com/foaf/0.1/Person
<http://xmlns.com/foaf/0.1/Person> rdf:type owl:Class .


###  https://w3id.org/aidoc-ap#AIDeployer
<https://w3id.org/aidoc-ap#AIDeployer> rdf:type owl:Class ;
                                       rdfs:subClassOf <http://www.w3.org/ns/prov#Agent> ,
                                                       <http://xmlns.com/foaf/0.1/Organization> ,
                                                       <https://w3id.org/aidoc-ap#AI_Agent> ;
                                       rdfs:comment "The entity that uses an AI system in a professional context."@en ;
                                       rdfs:label "AI Deployer"@en ;
                                       <http://www.w3.org/2004/02/skos/core#closeMatch> <https://w3id.org/vair#AIDeployer> .


###  https://w3id.org/aidoc-ap#AIProvider
<https://w3id.org/aidoc-ap#AIProvider> rdf:type owl:Class ;
                                       rdfs:subClassOf <http://www.w3.org/ns/prov#Agent> ,
                                                       <http://xmlns.com/foaf/0.1/Organization> ,
                                                       <https://w3id.org/aidoc-ap#AI_Agent> ;
                                       rdfs:comment "The entity that develops or places an AI system on the market."@en ;
                                       rdfs:label "AI Provider"@en ;
                                       <http://www.w3.org/2004/02/skos/core#closeMatch> <https://w3id.org/vair#AIProvider> .


###  https://w3id.org/aidoc-ap#AIResearcher
<https://w3id.org/aidoc-ap#AIResearcher> rdf:type owl:Class ;
                                         rdfs:subClassOf <http://www.w3.org/ns/prov#Agent> ,
                                                         <http://xmlns.com/foaf/0.1/Person> ,
                                                         <https://w3id.org/aidoc-ap#AI_Agent> ;
                                         rdfs:comment "A person involved in the technical development of an AI system."@en ;
                                         rdfs:label "AI Researcher"@en .


###  https://w3id.org/aidoc-ap#AI_Activity
<https://w3id.org/aidoc-ap#AI_Activity> rdf:type owl:Class ;
                                        rdfs:subClassOf <http://www.w3.org/ns/prov#Activity> ;
                                        rdfs:comment "A superclass for all activities in the AI lifecycle, derived from prov:Activity."@en ;
                                        rdfs:label "AI Activity"@en .


###  https://w3id.org/aidoc-ap#AI_Agent
<https://w3id.org/aidoc-ap#AI_Agent> rdf:type owl:Class ;
                                     rdfs:subClassOf <http://www.w3.org/ns/prov#Agent> ;
                                     rdfs:comment "A superclass for all agents involved in the AI lifecycle, derived from prov:Agent."@en ;
                                     rdfs:label "AI Agent"@en .


###  https://w3id.org/aidoc-ap#AI_Artifact
<https://w3id.org/aidoc-ap#AI_Artifact> rdf:type owl:Class ;
                                        rdfs:subClassOf <http://www.w3.org/ns/prov#Entity> ;
                                        rdfs:comment "A superclass for all tangible inputs and outputs of the AI lifecycle, derived from prov:Entity for provenance tracking."@en ;
                                        rdfs:label "AI Artifact"@en .


###  https://w3id.org/aidoc-ap#AI_Model
<https://w3id.org/aidoc-ap#AI_Model> rdf:type owl:Class ;
                                     rdfs:subClassOf <http://www.w3.org/ns/mls#Model> ,
                                                     <https://w3id.org/aidoc-ap#AI_Artifact> ;
                                     rdfs:comment "A computational representation that enables an AI method to execute an AI task."@en ;
                                     rdfs:label "AI Model"@en .


###  https://w3id.org/aidoc-ap#AISystem
<https://w3id.org/aidoc-ap#AISystem> rdf:type owl:Class ;
                                      rdfs:subClassOf <http://www.w3.org/ns/prov#Entity> ;
                                      rdfs:comment "The central entity representing the entire AI system."@en ;
                                      rdfs:label "AI System"@en ;
                                      <http://www.w3.org/2004/02/skos/core#closeMatch> <https://w3id.org/airo#AISystem> .


###  https://w3id.org/aidoc-ap#AIMethod
<https://w3id.org/aidoc-ap#AIMethod> rdf:type owl:Class ;
                                     rdfs:subClassOf <http://www.w3.org/ns/mls#Algorithm> ;
                                     rdfs:comment "Reflects a mathematical algorithm which computes input data to execute an AI task."@en ;
                                     rdfs:label "AI Method"@en .


###  https://w3id.org/aidoc-ap#Auditor
<https://w3id.org/aidoc-ap#Auditor> rdf:type owl:Class ;
                                    rdfs:subClassOf <http://www.w3.org/ns/prov#Agent> ,
                                                    <http://xmlns.com/foaf/0.1/Organization> ,
                                                    <http://xmlns.com/foaf/0.1/Person> ,
                                                    <https://w3id.org/aidoc-ap#AI_Agent> ;
                                    rdfs:comment "An organization or person responsible for reviewing the AI system for compliance."@en ;
                                    rdfs:label "Auditor"@en .


###  https://w3id.org/aidoc-ap#BuildAndIntegrationTesting
<https://w3id.org/aidoc-ap#BuildAndIntegrationTesting> rdf:type owl:Class ;
                                                       rdfs:subClassOf <https://w3id.org/aidoc-ap#SoftwareCodePipeline> ;
                                                       rdfs:comment "Activity of building system components and conducting integration testing."@en ;
                                                       rdfs:label "Build and Integration Testing"@en .


###  https://w3id.org/aidoc-ap#ChangeLog
<https://w3id.org/aidoc-ap#ChangeLog> rdf:type owl:Class ;
                                      rdfs:subClassOf <http://www.w3.org/ns/prov#Entity> ;
                                      rdfs:comment "A log of changes made to the system during its lifecycle."@en ;
                                      rdfs:label "Change Log"@en .


###  https://w3id.org/aidoc-ap#DataAcquisitionActivity
<https://w3id.org/aidoc-ap#DataAcquisitionActivity> rdf:type owl:Class ;
                                                    rdfs:subClassOf <https://w3id.org/aidoc-ap#DataPipeline> ;
                                                    rdfs:comment "The activity of obtaining data from various sources."@en ;
                                                    rdfs:label "Data Acquisition Activity"@en .


###  https://w3id.org/aidoc-ap#DataMonitoringAndLogging
<https://w3id.org/aidoc-ap#DataMonitoringAndLogging> rdf:type owl:Class ;
                                                     rdfs:subClassOf <https://w3id.org/aidoc-ap#DataPipeline> ;
                                                     rdfs:comment "Activity of capturing system events, performance, and traceability."@en ;
                                                     rdfs:label "Data Monitoring and Logging"@en .


###  https://w3id.org/aidoc-ap#DataPipeline
<https://w3id.org/aidoc-ap#DataPipeline> rdf:type owl:Class ;
                                         rdfs:subClassOf <https://w3id.org/aidoc-ap#AI_Activity> ;
                                         rdfs:comment "The pipeline for data-centric activities in the AI lifecycle."@en ;
                                         rdfs:label "Data Pipeline"@en .


###  https://w3id.org/aidoc-ap#DataTrainingAndTesting
<https://w3id.org/aidoc-ap#DataTrainingAndTesting> rdf:type owl:Class ;
                                                   rdfs:subClassOf <https://w3id.org/aidoc-ap#DataPipeline> ;
                                                   rdfs:comment "Activity of using datasets for model training, validation, and testing."@en ;
                                                   rdfs:label "Data Training and Testing"@en .


###  https://w3id.org/aidoc-ap#DataWrangling
<https://w3id.org/aidoc-ap#DataWrangling> rdf:type owl:Class ;
                                          rdfs:subClassOf <https://w3id.org/aidoc-ap#DataPipeline> ;
                                          rdfs:comment "Activity of ensuring data quality through cleaning, filtering, and enrichment."@en ;
                                          rdfs:label "Data Wrangling/Cleaning"@en .


###  https://w3id.org/aidoc-ap#Dataset
<https://w3id.org/aidoc-ap#Dataset> rdf:type owl:Class ;
                                    rdfs:subClassOf <http://mlcommons.org/croissant/1.0#Dataset> ,
                                                    <http://www.w3.org/ns/mls#Dataset> ,
                                                    <https://w3id.org/aidoc-ap#AI_Artifact> ;
                                    rdfs:comment "Represents a dataset used in the AI lifecycle."@en ;
                                    rdfs:label "Dataset"@en .


###  https://w3id.org/aidoc-ap#DeclarationOfConformity
<https://w3id.org/aidoc-ap#DeclarationOfConformity> rdf:type owl:Class ;
                                                    rdfs:subClassOf <http://www.w3.org/ns/prov#Entity> ;
                                                    rdfs:comment "A document declaring the system's conformity with standards, such as the EU Declaration of Conformity."@en ;
                                                    rdfs:label "Declaration of Conformity"@en .


###  https://w3id.org/aidoc-ap#Decommissioning
<https://w3id.org/aidoc-ap#Decommissioning> rdf:type owl:Class ;
                                            rdfs:subClassOf <https://w3id.org/aidoc-ap#SoftwareCodePipeline> ;
                                            rdfs:comment "Activity of taking a model out of production."@en ;
                                            rdfs:label "Decommissioning"@en .


###  https://w3id.org/aidoc-ap#Deployment
<https://w3id.org/aidoc-ap#Deployment> rdf:type owl:Class ;
                                       rdfs:subClassOf <https://w3id.org/aidoc-ap#SoftwareCodePipeline> ;
                                       rdfs:comment "Activity of delivering the AI system to production environments."@en ;
                                       rdfs:label "Deployment"@en .


###  https://w3id.org/aidoc-ap#ExplainableAIFeature
<https://w3id.org/aidoc-ap#ExplainableAIFeature> rdf:type owl:Class ;
                                                 rdfs:subClassOf <https://w3id.org/aidoc-ap#TransparencyMeasure> ;
                                                 rdfs:comment "A specific feature designed to provide explanations for the AI system's output."@en ;
                                                 rdfs:label "Explainable AI Feature"@en .


###  https://w3id.org/aidoc-ap#ExplorationAndValidation
<https://w3id.org/aidoc-ap#ExplorationAndValidation> rdf:type owl:Class ;
                                                     rdfs:subClassOf <https://w3id.org/aidoc-ap#DataPipeline> ;
                                                     rdfs:comment "Activity of reviewing data requirements, sources, and initial assessments."@en ;
                                                     rdfs:label "Exploration and Validation"@en .


###  https://w3id.org/aidoc-ap#HardwareComponent
<https://w3id.org/aidoc-ap#HardwareComponent> rdf:type owl:Class ;
                                              rdfs:subClassOf <http://www.w3.org/ns/prov#Entity> ;
                                              rdfs:comment "Represents the hardware required for an AI system to run."@en ;
                                              rdfs:label "Hardware Component"@en .


###  https://w3id.org/aidoc-ap#HumanOversightMechanism
<https://w3id.org/aidoc-ap#HumanOversightMechanism> rdf:type owl:Class ;
                                                    rdfs:subClassOf <http://www.w3.org/ns/prov#Entity> ;
                                                    rdfs:comment "A mechanism or measure to facilitate human intervention or supervision."@en ;
                                                    rdfs:label "Human Oversight Mechanism"@en .


###  https://w3id.org/aidoc-ap#Interface
<https://w3id.org/aidoc-ap#Interface> rdf:type owl:Class ;
                                      rdfs:subClassOf <http://www.w3.org/ns/prov#Entity> ;
                                      rdfs:comment "The interface provided for users or operators of an AI system."@en ;
                                      rdfs:label "Interface"@en .


###  https://w3id.org/aidoc-ap#Log
<https://w3id.org/aidoc-ap#Log> rdf:type owl:Class ;
                                rdfs:subClassOf <http://www.w3.org/ns/prov#Entity> ;
                                rdfs:comment "A record of system events, performance, and traceability."@en ;
                                rdfs:label "Log"@en .


###  https://w3id.org/aidoc-ap#ML_Pipeline
<https://w3id.org/aidoc-ap#ML_Pipeline> rdf:type owl:Class ;
                                        rdfs:subClassOf <https://w3id.org/aidoc-ap#AI_Activity> ;
                                        rdfs:comment "The pipeline for machine learning-centric activities in the AI lifecycle."@en ;
                                        rdfs:label "Machine Learning Pipeline"@en .


###  https://w3id.org/aidoc-ap#ModelEngineering
<https://w3id.org/aidoc-ap#ModelEngineering> rdf:type owl:Class ;
                                             rdfs:subClassOf <http://www.w3.org/ns/mls#Experiment> ,
                                                             <https://w3id.org/aidoc-ap#ML_Pipeline> ;
                                             rdfs:comment "Activity of defining architecture, selecting algorithms, and training the model."@en ;
                                             rdfs:label "Model Engineering"@en .


###  https://w3id.org/aidoc-ap#ModelEvaluation
<https://w3id.org/aidoc-ap#ModelEvaluation> rdf:type owl:Class ;
                                            rdfs:subClassOf <https://w3id.org/aidoc-ap#ML_Pipeline> ;
                                            rdfs:comment "Activity of assessing performance, robustness, and accuracy."@en ;
                                            rdfs:label "Model Evaluation"@en .


###  https://w3id.org/aidoc-ap#ModelPackaging
<https://w3id.org/aidoc-ap#ModelPackaging> rdf:type owl:Class ;
                                           rdfs:subClassOf <https://w3id.org/aidoc-ap#ML_Pipeline> ;
                                           rdfs:comment "Activity of preparing the trained model for deployment."@en ;
                                           rdfs:label "Model Packaging"@en .


###  https://w3id.org/aidoc-ap#ModelVersioning
<https://w3id.org/aidoc-ap#ModelVersioning> rdf:type owl:Class ;
                                            rdfs:subClassOf <https://w3id.org/aidoc-ap#ML_Pipeline> ;
                                            rdfs:comment "Activity of managing revisions and tracking changes in model iterations."@en ;
                                            rdfs:label "Model Versioning"@en .


###  https://w3id.org/aidoc-ap#PerformanceMetric
<https://w3id.org/aidoc-ap#PerformanceMetric> rdf:type owl:Class ;
                                              rdfs:subClassOf <http://www.w3.org/ns/dqv#Metric> ;
                                              rdfs:comment "A metric used to evaluate the performance of an AI system."@en ;
                                              rdfs:label "Performance Metric"@en .


###  https://w3id.org/aidoc-ap#PostMarketMonitoringActivity
<https://w3id.org/aidoc-ap#PostMarketMonitoringActivity> rdf:type owl:Class ;
                                                         rdfs:subClassOf <https://w3id.org/aidoc-ap#AI_Activity> ;
                                                         rdfs:comment "Activity of monitoring the system's performance and behavior after deployment."@en ;
                                                         rdfs:label "Post-market Monitoring Activity"@en .


###  https://w3id.org/aidoc-ap#PostMarketPerformanceEvaluationActivity
<https://w3id.org/aidoc-ap#PostMarketPerformanceEvaluationActivity> rdf:type owl:Class ;
                                                                    rdfs:subClassOf <https://w3id.org/aidoc-ap#AI_Activity> ;
                                                                    rdfs:comment "Activity of evaluating system performance in the post-market phase."@en ;
                                                                    rdfs:label "Post-market Performance Evaluation Activity"@en .


###  https://w3id.org/aidoc-ap#SoftwareCodePipeline
<https://w3id.org/aidoc-ap#SoftwareCodePipeline> rdf:type owl:Class ;
                                                 rdfs:subClassOf <https://w3id.org/aidoc-ap#AI_Activity> ;
                                                 rdfs:comment "The pipeline for software development-centric activities in the AI lifecycle."@en ;
                                                 rdfs:label "Software Code Pipeline"@en .


###  https://w3id.org/aidoc-ap#SoftwareDependency
<https://w3id.org/aidoc-ap#SoftwareDependency> rdf:type owl:Class ;
                                               rdfs:subClassOf <http://www.w3.org/ns/mls#Software> ,
                                                               <http://www.w3.org/ns/prov#Entity> ;
                                               rdfs:comment "A software package or library that the AI system depends on."@en ;
                                               rdfs:label "Software Dependency"@en .


###  https://w3id.org/aidoc-ap#SoftwareImplementation
<https://w3id.org/aidoc-ap#SoftwareImplementation> rdf:type owl:Class ;
                                                   rdfs:subClassOf <http://www.w3.org/ns/mls#Implementation> ,
                                                                   <https://w3id.org/aidoc-ap#AI_Artifact> ;
                                                   rdfs:comment "Represents the concrete, executable software that realizes an algorithm."@en ;
                                                   rdfs:label "Software Implementation"@en .


###  https://w3id.org/aidoc-ap#Standard
<https://w3id.org/aidoc-ap#Standard> rdf:type owl:Class ;
                                     rdfs:subClassOf <http://www.w3.org/ns/prov#Entity> ;
                                     rdfs:comment "A harmonised or other standard applied to the AI system."@en ;
                                     rdfs:label "Standard"@en ;
                                     <http://www.w3.org/2004/02/skos/core#closeMatch> <https://tair.adaptcentre.ie/documentation/tair_documentation.html#Standard> .


###  https://w3id.org/aidoc-ap#TransparencyMeasure
<https://w3id.org/aidoc-ap#TransparencyMeasure> rdf:type owl:Class ;
                                                rdfs:subClassOf <http://www.w3.org/ns/prov#Entity> ;
                                                rdfs:comment "A feature or measure to ensure the transparency of an AI system."@en ;
                                                rdfs:label "Transparency Measure"@en .


###  https://w3id.org/airo#AIRisk
<https://w3id.org/airo#AIRisk> rdf:type owl:Class .



#################################################################
#    Individuals
#################################################################
### Hierarchical Modeling ###
# Top-level categories as subclasses and SKOS concepts
<https://w3id.org/aidoc-ap#TraditionalAI> a <https://w3id.org/aidoc-ap#AIMethodCategory> ;
    rdfs:label "Traditional AI Techniques" ;
    skos:broader <https://w3id.org/aidoc-ap#AIMethodCategory> ;
    skos:definition "Algorithmic strategies for search, optimization, planning and decision making" .

<https://w3id.org/aidoc-ap#SymbolicAI> a <https://w3id.org/aidoc-ap#AIMethodCategory> ;
    rdfs:label "Symbolic AI" ;
    skos:broader <https://w3id.org/aidoc-ap#AIMethodCategory> ;
    skos:definition "Methods that use knowledge representation and logic-based reasoning to model knowledge and make inferences." .

<https://w3id.org/aidoc-ap#MachineLearning> a <https://w3id.org/aidoc-ap#AIMethodCategory> ;
    rdfs:label "Machine Learning" ;
    skos:broader <https://w3id.org/aidoc-ap#AIMethodCategory> ;
    skos:definition "Methods that learn patterns from data, including supervised, unsupervised, semi-supervised, self-supervised, and reinforcement learning." .

<https://w3id.org/aidoc-ap#HybridLearning> a <https://w3id.org/aidoc-ap#AIMethodCategory> ;
    rdfs:label "Hybrid Learning" ;
    skos:broader <https://w3id.org/aidoc-ap#AIMethodCategory> ;
    skos:definition "Methods that combine different learning paradigms, such as hybrid neuronal systems, learning with knowledge, and conversational learning." .


### Second-level descriptors under Traditional AI
<https://w3id.org/aidoc-ap#Search> a <https://w3id.org/aidoc-ap#AIMethodCategory> ;
    rdfs:label "Search" ;
    skos:broader <https://w3id.org/aidoc-ap#TraditionalAI> ;
    skos:definition "Techniques for exploring state spaces to find solutions." .

<https://w3id.org/aidoc-ap#Optimization> a <https://w3id.org/aidoc-ap#AIMethodCategory> ;
    rdfs:label "Optimization" ;
    skos:broader <https://w3id.org/aidoc-ap#TraditionalAI> ;
    skos:definition "Methods for improving solutions iteratively, including heuristic and metaheuristic approaches." .

<https://w3id.org/aidoc-ap#Planning> a <https://w3id.org/aidoc-ap#AIMethodCategory> ;
    rdfs:label "Planning" ;
    skos:broader <https://w3id.org/aidoc-ap#TraditionalAI> ;
    skos:definition "Approaches for autonomous and semi-autonomous planning procedures as well as plan recognition." .

<https://w3id.org/aidoc-ap#DecisionMaking> a <https://w3id.org/aidoc-ap#AIMethodCategory> ;
    rdfs:label "Decision Making" ;
    skos:broader <https://w3id.org/aidoc-ap#TraditionalAI> ;
    skos:definition "Approaches for selecting optimal actions under constraints or uncertainty." .

### Second-level descriptors under Symbolic AI
<https://w3id.org/aidoc-ap#KnowledgeRepresentation> a <https://w3id.org/aidoc-ap#AIMethodCategory> ;
    rdfs:label "Knowledge Representation" ;
    skos:broader <https://w3id.org/aidoc-ap#SymbolicAI> ;
    skos:definition "Methods for structuring and organizing knowledge, including ontologies, semantic networks, and knowledge graphs." . 

<https://w3id.org/aidoc-ap#LogicalReasoning> a <https://w3id.org/aidoc-ap#AIMethodCategory> ;
    rdfs:label "Logical Reasoning" ;
    skos:broader <https://w3id.org/aidoc-ap#SymbolicAI> ;
    skos:definition "Methods that use rules and principles for formal as well as interactive verification to identify patterns and logical structures and make logical deductions." .  

<https://w3id.org/aidoc-ap#ProbabilisticReasoning> a <https://w3id.org/aidoc-ap#AIMethodCategory> ;
    rdfs:label "Probabilistic Reasoning" ;
    skos:broader <https://w3id.org/aidoc-ap#SymbolicAI> ;
    skos:definition "Techniques that handle uncertainty and incomplete information using probabilistic models, such as Bayesian networks and Markov decision processes." .

<https://w3id.org/aidoc-ap#NonProbabilisticReasoning> a <https://w3id.org/aidoc-ap#AIMethodCategory> ;
    rdfs:label "Non-Probabilistic Reasoning" ;
    skos:broader <https://w3id.org/aidoc-ap#SymbolicAI> ;
    skos:definition "Techniques that do not rely on probabilistic models, such as qualitative procedures, rule-based approaches, reasoning with uncertainty as well as reasoning with belief functions." .

### Second-level descriptors under Machine Learning
<https://w3id.org/aidoc-ap#SupervisedLearning> a <https://w3id.org/aidoc-ap#AIMethodCategory> ;
    rdfs:label "Supervised Learning" ;
    skos:broader <https://w3id.org/aidoc-ap#MachineLearning> ;
    skos:definition "Techniques that learn from labeled data to make predictions or classifications." .

<https://w3id.org/aidoc-ap#UnsupervisedLearning> a <https://w3id.org/aidoc-ap#AIMethodCategory> ;
    rdfs:label "Unsupervised Learning" ;
    skos:broader <https://w3id.org/aidoc-ap#MachineLearning> ;
    skos:definition "Techniques that identify patterns and structures in unlabeled data." .

<https://w3id.org/aidoc-ap#SemiSupervisedLearning> a <https://w3id.org/aidoc-ap#AIMethodCategory> ;
    rdfs:label "Semi-Supervised Learning" ;
    skos:broader <https://w3id.org/aidoc-ap#MachineLearning> ;
    skos:definition "Techniques that combine a small amount of labeled data with a large amount of unlabeled data during training." .

<https://w3id.org/aidoc-ap#SelfSupervisedLearning> a <https://w3id.org/aidoc-ap#AIMethodCategory> ;
    rdfs:label "Self-Supervised Learning" ;
    skos:broader <https://w3id.org/aidoc-ap#MachineLearning> ;
    skos:definition "Techniques that generate their own labels from the input data to learn useful representations." .

<https://w3id.org/aidoc-ap#ReinforcementLearning> a <https://w3id.org/aidoc-ap#AIMethodCategory> ;
    rdfs:label "Reinforcement Learning" ;
    skos:broader <https://w3id.org/aidoc-ap#MachineLearning> ;
    skos:definition "Techniques that learn optimal actions through trial and error by receiving feedback in the form of rewards or penalties." .   

### Second-level descriptors under Supervised Learning
<https://w3id.org/aidoc-ap#Classification> a <https://w3id.org/aidoc-ap#AIMethodCategory> ;
    rdfs:label "Classification" ;
    skos:broader <https://w3id.org/aidoc-ap#SupervisedLearning> ;
    skos:definition "Techniques that assign input data to predefined categories or classes." .

<https://w3id.org/aidoc-ap#Regression> a <https://w3id.org/aidoc-ap#AIMethodCategory> ;
    rdfs:label "Regression" ;
    skos:broader <https://w3id.org/aidoc-ap#SupervisedLearning> ;
    skos:definition "Techniques that predict continuous output values based on input data." .

### Second-level descriptors under Unsupervised Learning
<https://w3id.org/aidoc-ap#Clustering> a <https://w3id.org/aidoc-ap#AIMethodCategory> ;
    rdfs:label "Clustering" ;
    skos:broader <https://w3id.org/aidoc-ap#UnsupervisedLearning> ;
    skos:definition "Techniques that group similar data points together based on their features." .

<https://w3id.org/aidoc-ap#DimensionReduction> a <https://w3id.org/aidoc-ap#AIMethodCategory> ;
    rdfs:label "Dimension Reduction" ;
    skos:broader <https://w3id.org/aidoc-ap#UnsupervisedLearning> ;
    skos:definition "Techniques that reduce the number of features in the data while preserving important information." .

### Second-level descriptors under Semi-Supervised Learning
<https://w3id.org/aidoc-ap#GraphBasedSemiSupervisedLearning> a <https://w3id.org/aidoc-ap#AIMethodCategory> ;
    rdfs:label "Graph-Based Semi-Supervised Learning" ;
    skos:broader <https://w3id.org/aidoc-ap#SemiSupervisedLearning> .

<https://w3id.org/aidoc-ap#StatisticalApproaches> a <https://w3id.org/aidoc-ap#AIMethodCategory> ;
    rdfs:label "Statistical Approaches" ;
    skos:broader <https://w3id.org/aidoc-ap#SemiSupervisedLearning> .

<https://w3id.org/aidoc-ap#ModifiedLearningConcepts> a <https://w3id.org/aidoc-ap#AIMethodCategory> ;
    rdfs:label "Modified Learning Concepts" ;
    skos:broader <https://w3id.org/aidoc-ap#SemiSupervisedLearning> .

### Second-level descriptors under Reinforcement Learning
<https://w3id.org/aidoc-ap#ModelFreeReinforcementLearning> a <https://w3id.org/aidoc-ap#AIMethodCategory> ;
    rdfs:label "Model-Free Reinforcement Learning" ;
    skos:broader <https://w3id.org/aidoc-ap#ReinforcementLearning> .

<https://w3id.org/aidoc-ap#ModelBasedReinforcementLearning> a <https://w3id.org/aidoc-ap#AIMethodCategory> ;
    rdfs:label "Model-Based Reinforcement Learning" ;
    skos:broader <https://w3id.org/aidoc-ap#ReinforcementLearning> .

### Second-level descriptors under Hybrid Learning
<https://w3id.org/aidoc-ap#HybridNeuronalSystems> a <https://w3id.org/aidoc-ap#AIMethodCategory> ;
    rdfs:label "Hybrid Neuronal Systems" ;
    skos:broader <https://w3id.org/aidoc-ap#HybridLearning> ;
    skos:definition "Methods that combine neural architectures with symbolic reasoning or other AI techniques." .

<https://w3id.org/aidoc-ap#LearningWithKnowledge> a <https://w3id.org/aidoc-ap#AIMethodCategory> ;
    rdfs:label "Learning with Knowledge" ;
    skos:broader <https://w3id.org/aidoc-ap#HybridLearning> ;
    skos:definition "Techniques that integrate both symbolic or explicit knowledge representation and machine learning approaches." .

<https://w3id.org/aidoc-ap#ConversationalLearning> a <https://w3id.org/aidoc-ap#AIMethodCategory> ;
    rdfs:label "Conversational Learning" ;
    skos:broader <https://w3id.org/aidoc-ap#HybridLearning> ;
    skos:definition "Methods that involve interactive learning through dialogue or feedback from users or other agents." .


###  First-level descriptors under AISystemCapability
<https://w3id.org/aidoc-ap#SensoryInputProcessing> a <https://w3id.org/aidoc-ap#AISystemCapability> ;
    rdfs:label "Sensory Input Processing" ;
    skos:broader <https://w3id.org/aidoc-ap#AISystemCapability> ;
    skos:definition "Internal sensory processing refers to AI system capabilities for interpreting data about its own internal states, such as position, orientation, pose, spatial configuration, or physical integrity, enabling self-monitoring and maintaining stability or optimal functioning." .

<https://w3id.org/aidoc-ap#KnowledgeProcessing> a <https://w3id.org/aidoc-ap#AISystemCapability> ;
    rdfs:label "Knowledge Processing" ;
    skos:broader <https://w3id.org/aidoc-ap#AISystemCapability> ;
    skos:definition "Knowledge processing refers to AI system capabilities for handling different types of knowledge—factual, conceptual, procedural, and metacognitive—through activities such as recognizing patterns, classifying information, generating concepts, executing procedures, and applying reflective reasoning to solve problems and adapt to new situations." .

<https://w3id.org/aidoc-ap#ActionControlProcessing> a <https://w3id.org/aidoc-ap#AISystemCapability> ;
    rdfs:label "Action Control Processing" ; 
    skos:broader <https://w3id.org/aidoc-ap#AISystemCapability> ;
    skos:definition "Action control processing refers to AI system capabilities that enable movement and control through mechanical, electronic, or software components, allowing simulation and execution of human-like behaviors, object manipulation, and natural gestures with high precision." .

<https://w3id.org/aidoc-ap#CommunicationProcessing> a <https://w3id.org/aidoc-ap#AISystemCapability> ;
    rdfs:label "Communication Processing" ;
    skos:broader <https://w3id.org/aidoc-ap#AISystemCapability> ;
    skos:definition "Communication processing encompasses AI system capabilities for transmitting and exchanging information, either unidirectionally without feedback or bidirectionally and omnidirectionally with feedback, enabling content generation and interactive communication in individual or group contexts." .
